RunTime/src/Monadic.lean
@@ -1,0 +1,84 @@
+import data.list.sort
+
+-- set_option trace.eqn_compiler.elim_match true
+
+universe variables u v
+variables {α : Type} (r : α → α → Prop) [decidable_rel r]
+local infix ` ≼ ` : 50 := r
+
+namespace timeMonad
+
+    inductive Timed (A : Sort u) (n : ℕ) : Sort (u + 1)
+    | box : A → Timed
+
+    open Timed
+
+    infixl ` inTime `:55 := Timed
+
+    @[simp] def untime {n : ℕ} {A : Sort u} : A inTime n → A
+    | (box a) := a
+
+    def bind {A : Sort u} {B : Sort v} {n m : ℕ} : A inTime n → (A → B inTime m) → B inTime (n + m)
+    | (box a) f := box (untime (f a))
+
+    def pure {A : Sort u} : A → A inTime 0 := box
+
+    infixl ` >>= `:55 := bind
+
+    def fmap {A : Sort u} {B : Sort v} {n : ℕ} : (A → B) → A inTime n → B inTime n
+    | f (box a) := box (f a)
+infixl ` <$> `:55 := fmap
+
+    def eqBound {A : Sort u} {n m : ℕ} : (n = m) → A inTime n → A inTime m
+    | _ (box a) := box a
+
+    def relaxBound {A : Sort u} {n m : ℕ} : (n ≤ m) → A inTime n → A inTime m
+    | _ (box a) := box a
+
+    axiom timedQuery' : ∀ (a b : α), psum (r a b) (r b a) inTime 1
+
+end timeMonad
+
+open timeMonad
+
+namespace insertionSort
+
+/- theorem ff : ∀ {A : Sort u} (a : A),  untime (pure a) = a := -/
+/- begin -/
+/-   intros, -/
+  
+/- end -/
+
+noncomputable def insert (a : α) : Π (xs : list α) , list α inTime xs.length
+| []         := pure [a]
+| (x :: xs') := have eqProof : (1 + xs'.length = (x :: xs').length),
+                by { simp, exact add_comm 1 xs'.length, },
+  eqBound eqProof $ timedQuery' r a x >>= λ cmp,
+                   match cmp with
+                     | (psum.inl ax) := relaxBound bot_le $ pure (a :: x :: xs')
+                     | (psum.inr xa) := (λ z , x :: z) <$> insert xs'
+                   end
+ 
+noncomputable def insertion_sort : Π (xs : list α) , list α inTime (xs.length * xs.length)
+| []         := pure []
+| (x :: xs') := have time_bound: xs'.length * xs'.length ≤ (x :: xs').length * xs'.length,
+                by { simp, rw mul_comm (xs'.length + 1) xs'.length, exact le_self_add, },
+  relaxBound time_bound (insertion_sort xs') >>=
+                (λ sorted_xs' , 
+                  let same_lengths : sorted_xs'.length = xs'.length := sorry,
+                      cons_inc_size: xs'.length ≤ (x :: xs').length := nat.le.intro rfl
+                  in relaxBound cons_inc_size (eqBound same_lengths (insert r x sorted_xs')))
+                 
+theorem insertion_sort_preserves_length :
+  ∀ (xs : list α), xs.length = (untime (insertion_sort r xs)).length
+| [] := begin simp, unfold insertion_sort, unfold timeMonad.pure, refl,  end
+| (x :: xs') :=
+begin
+  simp,
+  have ih := insertion_sort_preserves_length xs',
+  cases insertion_sort r (x :: xs') with sorted_xs',
+  simp,
+  sorry,
+end
+
+end insertionSort
